\section{Project: Gallagher's theorem}

\begin{lemma}
    \label{lem:gallagher1}
    Let $G$ be a finite group and 
    $N$ be a normal subgroup of $G$. Let $\psi\in\Irr(N)$ be such that
    $I_G(\psi)=G$. Then
    \[
    \Ind_N^G\psi=\sum_{\chi\in\Irr(G)}e_\chi\chi,
    \]
    where $e_\chi=\langle\Res_N^G,\chi\rangle$.
    In particular, 
    \[
    \sum_{\chi\in\Irr(G)}e_\chi^2=(G:N).
    \]
\end{lemma}

\begin{proof}
    Write $\Ind_N^G\psi$ as 
    \[
    \Ind_N^G\psi=\sum_{\chi\in\Irr(G)}e_\chi\chi,
    \]
    where by Frobenius' reciprocity $e_\chi=\langle\chi,\Ind_N^G\psi\rangle=\langle\Res_N^G\chi,\psi\rangle$.
    On the one hand, by Clifford's theorem, $\Res_N^G\chi=e_\chi\psi$ (because $I_G(\psi)=G$). In particular, 
    \[
    \chi(1)=(\Res_N^G\chi)(1)=e_\chi\psi(1).
    \]
    On the other hand, 
    \[
    (G:N)\psi(1)=(\Ind_N^G\psi)(1)=\sum_{\chi\in\Irr(G)}\langle\chi,\Ind_N^G\psi\rangle\chi(1)
    =\sum_{\chi\in\Irr(G)}e_\chi\chi(1)
    =\sum_{\chi\in\Irr(G)}e_\chi^2\psi(1).
    \]
    Since $\psi(1)\ne0$, it follows that  $(G:N)=\sum_{\chi\in\Irr(G)}e_\chi^2$. 
\end{proof}

\begin{lemma}
    \label{lem:Gallagher_reg}
    Let $G$ be a finite group and $N$ be a normal subgroup of $G$. Let... Then 
    \[
    \chi_L\chi=\Ind_N^G\Res_N^G\chi,
    \]    
    where $\chi_L$ is the character of the regular representation of $G/N$. 
\end{lemma}

\begin{proof}
    On the one hand, in the proof of Theorem~\ref{thm:regular} we have seen a formula to compute
    the values of the character of the regular representation of a group. In our case, 
    \[
    \chi_L(g)=\begin{cases}
        (G:N) & \text{if $g\in N$},\\
        0 & \text{otherwise}.
    \end{cases}
    \]
    On the other hand, 
    \begin{align*}
        (\Ind_N^G\Res_N^G)(g) &= \frac{1}{|N|}\sum_{x\in G}(\Res_N^G\chi)^0(x^{-1}gx).
    \end{align*}
    Note that $x^{-1}gx\in N$ if and only if $g\in xNx^{-1}=N$. Thus if $g\not\in N$, then
    $(\Ind_N^G\Res_N^G)(g)=0$ and this coincides with $\chi_L(g)\chi(g)$, since $\chi_L(g)=0$. Suppose 
    then that $g\in N$. Then 
    \[
    (\Ind_N^G\Res_N^G)(g)=\frac{1}{|N|}\sum_{x\in G}\chi(g)=(G:N)\chi(g)=\chi_L(g)\chi(g).\qedhere 
    \]
\end{proof}

\begin{theorem}[Gallagher]
\label{thm:Gallagher}
\index{Gallagher theorem}
    Let $G$ be a finite group and $N$ be a normal subgroup of $G$. 
    Let $\chi\in\Irr(G)$ be such that $\psi=\Res_N^G\chi\in\Irr(N)$. Then
    \[
    \Ind_N^G\psi=\sum_{\lambda\in\Irr(G/N)}\lambda(1)(\Inf_{G/N}^G\lambda)\chi,
    \]
    where the characters $(\Inf_{G/N}^G\lambda)\chi$ are pairwise different and irreducible. 
\end{theorem}

\begin{proof}
    Since $\psi=\Res_N^G\chi$, Lemma~\ref{lem:Gallagher_reg} implies that 
    \[
    \Ind_N^G\psi=\Ind_N^G\Res_N^G\chi=(\Inf_{G/N}^G\xi)\chi,
    \]
    where $\xi$ is the character of the regular representation of $G/N$. In the proof
    of Theorem~\ref{thm:regular} we have seen that
    \[
    \xi=\sum_{\lambda\in\Irr(G/N)}\lambda(1)\lambda. 
    \]
    By Lemma~\ref{lem:gallagher1}, 
    \begin{align*}
        (G:N)&=\sum_{\chi\in\Irr(G)}e_\chi^2
        =\langle\Ind_N^G\psi,\Ind_N^G\psi\rangle\\
        &=\sum_{\lambda,\mu\in\Irr(G/N)}\lambda(1)\mu(1)\langle\Inf_{G/N}^G\lambda,\Inf_{G/N}^G\mu\rangle
        \geq\sum_{\lambda\in\Irr(G/N)}\lambda(1)^2=(G:N).        
    \end{align*}
    It follows that 
    \[
    \langle\Inf_{G/N}^G\lambda,\Inf_{G/N}^G\mu\rangle=\begin{cases}
        1 & \text{if $\lambda=\mu$,}\\
        0 & \text{otherwise.}
    \end{cases}
    \]
    In particular, the characters...
\end{proof}

\begin{exercise}
    Let $G$ be a finite group and $N$ be a normal subgroup of $G$. Let $\chi\in\Irr(G)$ 
    be such that $\theta=\Res_N^G\chi\in\Irr(N)$. Prove that the map 
    $\psi\mapsto(\Inf_{G/N}^G\psi)\chi$ yields 
    a bijective 
    correspondence 
    \[
    \Irr(G/N)\leftrightarrow\{\eta\in\Irr(G):\langle\Res_N^G\eta,\theta\rangle>0\}.
    \]
\end{exercise}